theories/Core/Soundness/Weakening/Definitions.v
@@ -12,7 +12,7 @@ Inductive weakening {P : PtsSig} : ctx P -> sub P -> ctx P -> Prop :=
   `( {{ Γ ⊢s σ ≈ Id : Δ }} ->
      {{ Γ ⊢w σ : Δ }} )
 | wk_p :
-  `( {{ Γ ⊢w τ : Δ', A@s }} ->
+  `( {{ Γ ⊢w τ : Δ', A }} ->
      {{ ⊢ Δ' ⊆ Δ }} ->
      {{ Γ ⊢s σ ≈ Wk ∘ τ : Δ }} ->
      {{ Γ ⊢w σ : Δ }} )
